writing Stub.v
--HG--
branch : adt

platform/cito/CompileModule.v
@@ -2,6 +2,7 @@ Require Import SyntaxModule.
 Require Import List.
 Require CompileFunc.
 Require Import GoodFunc GoodOptimizer.
+Require Import GoodModule.
 
 Set Implicit Arguments.
 
@@ -35,17 +36,9 @@ Definition NoDupFuncNames mod_name funcs :=
 
 Section TopSection.
 
-  Variable module : CitoModule.
+  Variable module : GoodModule.
 
   Require Import CompileFuncImpl.
-  Record GoodModule module := 
-    {
-      NoDupFuncNames_ : NoDup (map Name (Functions module));
-      GoodFuncs : List.Forall GoodFunc (Functions module)
-    }.
-
-  Hypothesis good_module : GoodModule module.
-
   Require Import StructuredModule.
   Definition imports : list import := nil.
 
@@ -53,22 +46,17 @@ Section TopSection.
 
   Hypothesis good_optimizer : GoodOptimizer optimizer.
 
-  Definition to_prod_list : forall A P (ls : list A), List.Forall P ls -> list { x | P x }.
-    induction ls.
-    econstructor 1.
-    econstructor 2.
-    econstructor; inversion H; subst; eauto.
-    eapply IHls; inversion H; subst; eauto.
-  Defined.
+  Require Import NameDecoration.
+  Definition mod_name := impl_module_name (Name module).
 
-  Definition compile_func' f (good_func : GoodFunc f) := CompileFunc.compile (ModuleName module) good_func good_optimizer.
+  Definition compile_func' f (good_func : GoodFunc f) := CompileFunc.compile mod_name good_func good_optimizer.
 
   Definition compile_func (p : { f | GoodFunc f }) :=
     match p with
       | exist _ good_func => compile_func' good_func
     end.
 
-  Definition compiled_funcs := map compile_func (to_prod_list (GoodFuncs good_module)).
+  Definition compiled_funcs := map compile_func (Functions module).
 
   Require Import Structured.
   Require Import Wrap.
@@ -78,7 +66,7 @@ Section TopSection.
 
   Definition compile := StructuredModule.bmodule_ imports compiled_funcs.
 
-  Lemma module_name_not_in_imports : NameNotInImports (ModuleName module) imports.
+  Lemma module_name_not_in_imports : NameNotInImports mod_name imports.
     unfold NameNotInImports; eauto.
   Qed.
 
