platform/cito/Label.v
@@ -1,0 +1,28 @@
+Require Import FMapWeakList.
+Require Import String.
+Require Import Equalities.
+
+Set Implicit Arguments.
+
+Definition label := (string * string)%type.
+
+Module Key <: MiniDecidableType.
+  Definition t := label.
+  Definition eq_dec (a b : label) : {a = b} + {a <> b}.
+    destruct a.
+    destruct b.
+    destruct (string_dec s s1).
+    destruct (string_dec s0 s2).
+    left.
+    congruence.
+    right.
+    congruence.
+    right.
+    congruence.
+  Defined.
+End Key.
+
+Module Key' := Make_UDT Key.
+Module LabelMap := Make Key'.
+
+
